theories/Bind.v
@@ -1,0 +1,537 @@
+(**
+
+This file describes the representation of variables, binders, and
+contexts.
+
+Author: Arthur Charguéraud.
+License: MIT.
+
+*)
+
+Set Implicit Arguments.
+From TLC Require Export LibString LibList LibCore.
+From Sep Require Export Fmap TLCbuffer.
+Open Scope string_scope.
+
+
+(* ********************************************************************** *)
+(* * Variables *)
+
+(* ---------------------------------------------------------------------- *)
+(** Representation of variables *)
+
+(** Variables are represented as strings *)
+
+Definition var := string.
+
+(** Variables can be compared via [var_eq s1 s2] *)
+
+Definition eq_var_dec := String.string_dec.
+
+Definition var_eq (s1:var) (s2:var) : bool :=
+  if eq_var_dec s1 s2 then true else false.
+
+Lemma var_eq_spec : forall s1 s2,
+  var_eq s1 s2 = isTrue (s1 = s2).
+Proof using.
+  intros. unfold var_eq. case_if; rew_bool_eq~.
+Qed.
+
+Global Opaque var.
+
+(** Tactic [var_neq] for proving two concrete variables distinct.
+    Also registered as hint for [auto] *)
+
+Ltac var_neq :=
+  match goal with |- ?x <> ?y :> var =>
+    solve [ let E := fresh in
+            destruct (eq_var_dec x y) as [E|E];
+              [ false | apply E ] ] end.
+
+Hint Extern 1 (?x <> ?y) => var_neq.
+
+
+(* ---------------------------------------------------------------------- *)
+(** Distinct variables *)
+
+(** [vars] is the type of a list of variables *)
+
+Definition vars : Type := list var.
+
+(** [var_fresh y xs] asserts that [y] does not belong to the list [xs] *)
+
+Fixpoint var_fresh (y:var) (xs:vars) : bool :=
+  match xs with
+  | nil => true
+  | x::xs' => if var_eq x y then false else var_fresh y xs'
+  end.
+
+(** [var_distinct xs] asserts that [xs] consists of a list of distinct variables. *)
+
+Fixpoint var_distinct (xs:vars) : Prop :=
+  match xs with
+  | nil => True
+  | x::xs' => var_fresh x xs' /\ var_distinct xs'
+  end.
+
+(** Computable version of [var_distinct] *)
+
+Fixpoint var_distinct_exec (xs:vars) : bool :=
+  match xs with
+  | nil => true
+  | x::xs' => var_fresh x xs' && var_distinct_exec xs'
+  end.
+
+Lemma var_distinct_exec_eq : forall xs,
+  var_distinct_exec xs = isTrue (var_distinct xs).
+Proof using.
+  intros. induction xs as [|x xs']; simpl; rew_isTrue.
+  { auto. } { rewrite~ IHxs'. }
+Qed.
+
+
+(* ---------------------------------------------------------------------- *)
+(** Nonempty lists of [n] distinct variables *)
+
+(** [var_funs n xs] asserts that [xs] consists of [n] distinct variables *)
+
+Definition var_funs (n:nat) (xs:vars) : Prop :=
+     var_distinct xs
+  /\ length xs = n
+  /\ xs <> nil.
+
+(** [var_fixs f n xs] asserts that [f::xs] consists of [n+1]
+    distinct variables. *)
+
+Definition var_fixs (f:var) (n:nat) (xs:vars) : Prop :=
+     var_distinct (f::xs)
+  /\ length xs = n
+  /\ xs <> nil.
+
+(** Computable version of [var_funs] *)
+
+Definition var_funs_exec (n:nat) (xs:vars) : bool :=
+     nat_compare n (List.length xs)
+  && is_not_nil xs
+  && var_distinct_exec xs.
+
+Lemma var_funs_exec_eq : forall (n:nat) xs,
+  var_funs_exec n xs = isTrue (var_funs n xs).
+Proof using.
+  intros. unfold var_funs_exec, var_funs.
+  rewrite nat_compare_eq.
+  rewrite is_not_nil_eq.
+  rewrite List_length_eq.
+  rewrite var_distinct_exec_eq.
+  extens. rew_istrue. iff*.
+Qed.
+
+(** Computable version of [var_fixs] *)
+
+Definition var_fixs_exec (f:var) (n:nat) (xs:vars) : bool :=
+     nat_compare n (List.length xs)
+  && is_not_nil xs
+  && var_distinct_exec (f::xs).
+
+Lemma var_fixs_exec_eq : forall f (n:nat) xs,
+  var_fixs_exec f n xs = isTrue (var_fixs f n xs).
+Proof using.
+  intros. unfold var_fixs_exec, var_fixs.
+  rewrite nat_compare_eq.
+  rewrite is_not_nil_eq.
+  rewrite List_length_eq.
+  rewrite var_distinct_exec_eq.
+  extens. rew_istrue. iff*.
+Qed.
+
+
+(* ---------------------------------------------------------------------- *)
+(* ** Generation of n variables *)
+
+(** [nat_to_var n] converts [nat] values into distinct
+    [name] values.
+    Warning: the current implementation is inefficient. *)
+
+Definition dummy_char := Ascii.ascii_of_nat 0%nat.
+
+Fixpoint nat_to_var (n:nat) : var :=
+  match n with
+  | O => String.EmptyString
+  | S n' => String.String dummy_char (nat_to_var n')
+  end.
+
+Lemma injective_nat_to_var : injective nat_to_var.
+Proof using.
+  intros n. induction n as [|n']; intros m E; destruct m as [|m']; tryfalse.
+  { auto. }
+  { inverts E. fequals~. }
+Qed.
+
+(** [var_seq i n] generates a list of variables [x1;x2;..;xn]
+    with [x1=i] and [xn=i+n-1]. Such lists are useful for
+    generic programming. *)
+
+Fixpoint var_seq (start:nat) (nb:nat) : vars :=
+  match nb with
+  | O => nil
+  | S nb' => (nat_to_var start) :: var_seq (S start) nb'
+  end.
+
+(** Properties of [var_seq] follow *)
+
+Section Var_seq.
+Implicit Types start nb : nat.
+
+Lemma var_fresh_var_seq_lt : forall (x:nat) start nb,
+  (x < start)%nat ->
+  var_fresh (nat_to_var x) (var_seq start nb).
+Proof using.
+  intros. gen start. induction nb; intros.
+  { auto. }
+  { simpl. rewrite var_eq_spec. case_if.
+    { lets: injective_nat_to_var C. math. }
+    { applys IHnb. math. } }
+Qed.
+
+Lemma var_fresh_var_seq_ge : forall (x:nat) start nb,
+  (x >= start+nb)%nat ->
+  var_fresh (nat_to_var x) (var_seq start nb).
+Proof using.
+  intros. gen start. induction nb; intros.
+  { auto. }
+  { simpl. rewrite var_eq_spec. case_if.
+    { lets: injective_nat_to_var C. math. }
+    { applys IHnb. math. } }
+Qed.
+
+Lemma var_distinct_var_seq : forall start nb,
+  var_distinct (var_seq start nb).
+Proof using.
+  intros. gen start. induction nb; intros.
+  { simple~. }
+  { split.
+    { applys var_fresh_var_seq_lt. math. }
+    { auto. } }
+Qed.
+
+Lemma length_var_seq : forall start nb,
+  length (var_seq start nb) = nb.
+Proof using.
+  intros. gen start. induction nb; simpl; intros.
+  { auto. } { rew_list. rewrite~ IHnb. }
+Qed.
+
+Lemma var_funs_var_seq : forall start nb,
+  (nb > 0%nat)%nat ->
+  var_funs nb (var_seq start nb).
+Proof using.
+  introv E. splits.
+  { applys var_distinct_var_seq. }
+  { applys length_var_seq. }
+  { destruct nb. { false. math. } { simpl. auto_false. } }
+Qed.
+
+End Var_seq.
+
+
+
+(* ********************************************************************** *)
+(* * Binders *)
+
+(** A binder is either a variable or the anonymous binder. *)
+
+Inductive bind : Type :=
+  | bind_anon : bind
+  | bind_var : var -> bind.
+
+(** Variables and strinsg can be coerced to binders. *)
+
+Coercion bind_var : var >-> bind.
+Coercion bind_var' (x:string) : bind := bind_var x.
+
+
+
+(* ********************************************************************** *)
+(* * Contexts *)
+
+Module Ctx.
+
+(* ---------------------------------------------------------------------- *)
+(** Definition of contexts *)
+
+(** A context associate variables with values. *)
+
+(** [ctx] describes a list of bindings *)
+
+Definition ctx (A:Type) : Type :=
+  list (var * A).
+
+(* ---------------------------------------------------------------------- *)
+(** Operations of contexts *)
+
+(** [empty] describes the empty context *)
+
+Definition empty A : ctx A :=
+  @nil _.
+
+Arguments empty {A}.
+
+(** [add z v E] is defined as:
+    - [E] if [z] is the anonymous binder
+    - [E] extended with the pair [(x,v)] if [z] is a variable [x]. *)
+
+Definition add A (z:bind) (v:A) (E:ctx A) : ctx A :=
+  match z with
+  | bind_anon => E
+  | bind_var x => (x,v)::E
+  end.
+
+(** [one z v] is a shorthand for [add z v empty] *)
+
+Definition one A (z:bind) (v:A) : ctx A :=
+  add z v empty.
+
+(** [rem x E] removes all bindings on [x] stored in [E] *)
+
+Fixpoint rem_var A (x:var) (E:ctx A) : ctx A :=
+  match E with
+  | nil => nil
+  | (y,v)::E' =>
+      let E'' := rem_var x E' in
+      if var_eq x y then E'' else (y,v)::E''
+  end.
+
+Fixpoint rem A (z:bind) (E:ctx A) : ctx A :=
+  match z with
+  | bind_anon => E
+  | bind_var x => rem_var x E
+  end.
+
+(** [lookup x E] returns
+    - [None] if [x] is not bound in [E]
+    - [Some v] if [x] is bound to [v] in [E]. *)
+
+Fixpoint lookup A (x:var) (E:ctx A) : option A :=
+  match E with
+  | nil => None
+  | (y,v)::E' => if var_eq x y
+                   then Some v
+                   else lookup x E'
+  end.
+
+(** [fresh x E] asserts that [x] is not bound in [E] *)
+
+Definition fresh A (x:var) (E:ctx A) : Prop :=
+  lookup x E = None.
+
+
+(* ---------------------------------------------------------------------- *)
+(** Properties of operations on contexts *)
+
+Section CtxOps.
+Variables (A : Type).
+Implicit Type (E : ctx A).
+
+
+(* ---------------------------------------------------------------------- *)
+(** Lemmas to reintroduce contexts *)
+
+Lemma nil_eq_ctx_empty :
+  @nil (prod var A) = empty.
+Proof using. auto. Qed.
+
+Lemma cons_eq_ctx_add : forall x v E,
+  (x,v)::E = add x v E.
+Proof using. auto. Qed.
+
+
+(* ---------------------------------------------------------------------- *)
+(** Properties of operations on contexts  *)
+
+Lemma fresh_inv : forall (x1 x2:var) v E,
+  fresh x1 (add x2 v E) ->
+  x1 <> x2 /\ fresh x1 E.
+Proof using.
+  introv M. unfolds fresh. simpls.
+  rewrite var_eq_spec in *. case_if~.
+Qed.
+
+(** [rem x empty] *)
+
+Lemma rem_empty : forall z,
+  rem z (@empty A) = empty.
+Proof using. intros. destruct z as [|x]; auto. Qed.
+
+(** Result of removing a variable from a context. *)
+(* -- TODO: rename and check useful *)
+
+Lemma rem_add_same : forall z v E,
+  rem z (add z v E) = rem z E.
+Proof using.
+  intros. destruct z as [|x].
+  { auto. }
+  { simpl. rewrite var_eq_spec. case_if~. }
+Qed.
+
+Lemma rem_add_neq : forall z1 z2 v E,
+  z1 <> z2 ->
+  rem z1 (add z2 v E) = add z2 v (rem z1 E).
+Proof using.
+  intros. destruct z2 as [|x2].
+  { auto. }
+  { destruct z1 as [|x1].
+    { auto. }
+    { simpl. rewrite var_eq_spec. case_if~. } }
+Qed.
+
+(** Removing a variable that does not occur in a context changes nothing. *)
+
+Lemma rem_fresh : forall x E,
+  fresh x E ->
+  rem x E = E.
+Proof using.
+  introv M. unfold rem. induction E as [|(y,v) E'].
+  { auto. }
+  { simpls. lets (N1&N2): fresh_inv (rm M).
+    rewrite var_eq_spec in *. case_if. rewrite~ IHE'. }
+Qed.
+
+End CtxOps.
+
+End Ctx.
+
+(* LATER: how to place this rewrite base and tactics inside the
+   module and still be able to use it without importing the module? *)
+
+Hint Rewrite Ctx.nil_eq_ctx_empty Ctx.cons_eq_ctx_add : rew_ctx.
+
+Tactic Notation "rew_ctx" :=
+  autorewrite with rew_ctx.
+Tactic Notation "rew_ctx" "in" hyp(H) :=
+  autorewrite with rew_ctx in H.
+Tactic Notation "rew_ctx" "in" "*" :=
+  autorewrite with rew_ctx in *.
+
+
+
+(* ********************************************************************** *)
+(* * Notation for program variables *)
+
+(** To avoid using the string notation ["x"] for refering to a
+    variable called [x], one can use the notation ['x], available
+    by importing the following module. *)
+
+
+Module NotationForVariables.
+
+Notation "''a'" := ("a":var) : var_scope.
+Notation "''b'" := ("b":var) : var_scope.
+Notation "''c'" := ("c":var) : var_scope.
+Notation "''d'" := ("d":var) : var_scope.
+Notation "''e'" := ("e":var) : var_scope.
+Notation "''f'" := ("f":var) : var_scope.
+Notation "''g'" := ("g":var) : var_scope.
+Notation "''h'" := ("h":var) : var_scope.
+Notation "''i'" := ("i":var) : var_scope.
+Notation "''j'" := ("j":var) : var_scope.
+Notation "''k'" := ("k":var) : var_scope.
+Notation "''l'" := ("l":var) : var_scope.
+Notation "''m'" := ("m":var) : var_scope.
+Notation "''n'" := ("n":var) : var_scope.
+Notation "''o'" := ("o":var) : var_scope.
+Notation "''p'" := ("p":var) : var_scope.
+Notation "''q'" := ("q":var) : var_scope.
+Notation "''r'" := ("r":var) : var_scope.
+Notation "''s'" := ("s":var) : var_scope.
+Notation "''t'" := ("t":var) : var_scope.
+Notation "''u'" := ("u":var) : var_scope.
+Notation "''v'" := ("v":var) : var_scope.
+Notation "''w'" := ("w":var) : var_scope.
+Notation "''x'" := ("x":var) : var_scope.
+Notation "''y'" := ("y":var) : var_scope.
+Notation "''z'" := ("z":var) : var_scope.
+
+Notation "''a1'" := ("a1":var) : var_scope.
+Notation "''b1'" := ("b1":var) : var_scope.
+Notation "''c1'" := ("c1":var) : var_scope.
+Notation "''d1'" := ("d1":var) : var_scope.
+Notation "''e1'" := ("e1":var) : var_scope.
+Notation "''f1'" := ("f1":var) : var_scope.
+Notation "''g1'" := ("g1":var) : var_scope.
+Notation "''h1'" := ("h1":var) : var_scope.
+Notation "''i1'" := ("i1":var) : var_scope.
+Notation "''j1'" := ("j1":var) : var_scope.
+Notation "''k1'" := ("k1":var) : var_scope.
+Notation "''l1'" := ("l1":var) : var_scope.
+Notation "''m1'" := ("m1":var) : var_scope.
+Notation "''n1'" := ("n1":var) : var_scope.
+Notation "''o1'" := ("o1":var) : var_scope.
+Notation "''p1'" := ("p1":var) : var_scope.
+Notation "''q1'" := ("q1":var) : var_scope.
+Notation "''r1'" := ("r1":var) : var_scope.
+Notation "''s1'" := ("s1":var) : var_scope.
+Notation "''t1'" := ("t1":var) : var_scope.
+Notation "''u1'" := ("u1":var) : var_scope.
+Notation "''v1'" := ("v1":var) : var_scope.
+Notation "''w1'" := ("w1":var) : var_scope.
+Notation "''x1'" := ("x1":var) : var_scope.
+Notation "''y1'" := ("y1":var) : var_scope.
+Notation "''z1'" := ("z1":var) : var_scope.
+
+Notation "''a2'" := ("a2":var) : var_scope.
+Notation "''b2'" := ("b2":var) : var_scope.
+Notation "''c2'" := ("c2":var) : var_scope.
+Notation "''d2'" := ("d2":var) : var_scope.
+Notation "''e2'" := ("e2":var) : var_scope.
+Notation "''f2'" := ("f2":var) : var_scope.
+Notation "''g2'" := ("g2":var) : var_scope.
+Notation "''h2'" := ("h2":var) : var_scope.
+Notation "''i2'" := ("i2":var) : var_scope.
+Notation "''j2'" := ("j2":var) : var_scope.
+Notation "''k2'" := ("k2":var) : var_scope.
+Notation "''l2'" := ("l2":var) : var_scope.
+Notation "''m2'" := ("m2":var) : var_scope.
+Notation "''n2'" := ("n2":var) : var_scope.
+Notation "''o2'" := ("o2":var) : var_scope.
+Notation "''p2'" := ("p2":var) : var_scope.
+Notation "''q2'" := ("q2":var) : var_scope.
+Notation "''r2'" := ("r2":var) : var_scope.
+Notation "''s2'" := ("s2":var) : var_scope.
+Notation "''t2'" := ("t2":var) : var_scope.
+Notation "''u2'" := ("u2":var) : var_scope.
+Notation "''v2'" := ("v2":var) : var_scope.
+Notation "''w2'" := ("w2":var) : var_scope.
+Notation "''x2'" := ("x2":var) : var_scope.
+Notation "''y2'" := ("y2":var) : var_scope.
+Notation "''z2'" := ("z2":var) : var_scope.
+
+Notation "''a3'" := ("a3":var) : var_scope.
+Notation "''b3'" := ("b3":var) : var_scope.
+Notation "''c3'" := ("c3":var) : var_scope.
+Notation "''d3'" := ("d3":var) : var_scope.
+Notation "''e3'" := ("e3":var) : var_scope.
+Notation "''f3'" := ("f3":var) : var_scope.
+Notation "''g3'" := ("g3":var) : var_scope.
+Notation "''h3'" := ("h3":var) : var_scope.
+Notation "''i3'" := ("i3":var) : var_scope.
+Notation "''j3'" := ("j3":var) : var_scope.
+Notation "''k3'" := ("k3":var) : var_scope.
+Notation "''l3'" := ("l3":var) : var_scope.
+Notation "''m3'" := ("m3":var) : var_scope.
+Notation "''n3'" := ("n3":var) : var_scope.
+Notation "''o3'" := ("o3":var) : var_scope.
+Notation "''p3'" := ("p3":var) : var_scope.
+Notation "''q3'" := ("q3":var) : var_scope.
+Notation "''r3'" := ("r3":var) : var_scope.
+Notation "''s3'" := ("s3":var) : var_scope.
+Notation "''t3'" := ("t3":var) : var_scope.
+Notation "''u3'" := ("u3":var) : var_scope.
+Notation "''v3'" := ("v3":var) : var_scope.
+Notation "''w3'" := ("w3":var) : var_scope.
+Notation "''x3'" := ("x3":var) : var_scope.
+Notation "''y3'" := ("y3":var) : var_scope.
+Notation "''z3'" := ("z3":var) : var_scope.
+
+Open Scope var_scope.
+
+End NotationForVariables.
